src/tls/StreamPlain.fst
@@ -19,7 +19,7 @@ open Content
 type id = i:id { pv_of_id i = TLS_1p3 }  
 
 
-(***  plain := fragment | CT | 0*  ***)
+(*** plain := fragment | CT | 0*  ***)
 
 // naming: we switch from fragment to plain as we are no longer TLS-specific
 // similarly, the length accounts for the TLS-specific CT byte.
@@ -29,7 +29,7 @@ let plainLength (l:int) = 1 <= l /\ l <= max_TLSCiphertext_fragment_length_13
 type plainLen = l:nat { plainLength l }
 type plainRepr = b:bytes { plainLength (length b) }
 
-type plain (i:id) (len: plainLen) = f:fragment i { len = snd (Content.rg i f) + 1 }
+type plain (i:id) (len:plainLen) = f:fragment i { len >= snd (Content.rg i f) + 1 }
 
 let pad payload ct (len:plainLen { length payload < len }): plainRepr = 
   payload @| ctBytes ct @| createBytes (len - length payload - 1) 0z
@@ -40,55 +40,61 @@ let ghost_repr #i #len f =
   let payload = Content.ghost_repr #i f in 
   pad payload ct len
 
+// slight code duplication between monads; avoidable? 
 val repr: i:id{ ~(safeId i)} -> len: plainLen -> p:plain i len -> Tot (b:lbytes len {b = ghost_repr #i #len p})
 let repr i len f = 
   let ct,_ = ct_rg i f in 
   let payload = Content.repr i f in 
   pad payload ct len
 
-// slight code duplication between monads; avoidable? 
 
-(* 
-val scan: bs:bytes -> j: nat { j < length bs /\ (forall (k:nat {j < k /\ k < length bs}). Seq.index bs k = 0z) } -> 
-  Tot (o:option(j:nat { j < length bs /\ Seq.index bs j <> 0z /\ (forall (k:nat {j < k /\ k < length bs}). Seq.index bs k = 0z) }))
- 
-let rec scan bs j =
-  if Seq.index bs j <> 0z then Some j 
-  else if j = 0            then None 
-  else scan bs (j-1)
-*)
+// Implementations MUST NOT send zero-length fragments of Handshake,
+// Alert, or ChangeCipherSpec content types. Zero-length fragments of
+// Application data MAY be sent as they are potentially useful as a
+// traffic analysis countermeasure.
 
 val scan: i:id { ~ (authId i) } -> bs:plainRepr -> 
-  j: nat { j < length bs /\ 
+  j:nat { j < length bs /\ 
          (forall (k:nat {j < k /\ k < length bs}).{:pattern (Seq.index bs k)} Seq.index bs k = 0z) } -> 
-  Tot(result(p:plain i (length bs) { bs = ghost_repr #i #(length bs) p }))
+  Tot (result (p:plain i (length bs) { bs = ghost_repr #i #(length bs) p }))
 let rec scan i bs j =
   let len = length bs in 
-  let v = index bs j in 
-  if j > max_TLSPlaintext_fragment_length + 1 then 
-    // the CT byte cannot be beyond the largest plaintext length; so those bytes must be 0z
-    if v = 0z then scan i bs (j-1) 
-    else Error (AD_decode_error, "")  //TODO pick better error
-  else 
-  match v with 
-  | 0z  -> if j > 0 then scan i bs (j-1) 
-          else Error (AD_decode_error, "") 
-  | 21z -> let rg: frange i = (0, j) in
-           let payload, rest = Platform.Bytes.split bs j in 
-           let f = CT_Alert rg payload in 
-           lemma_eq_intro bs (pad payload Alert len);
-           Correct f
-  | 22z -> let rg:frange i = (0, j) in
-           let payload = fst (Platform.Bytes.split bs j) in 
-           let f = CT_Handshake rg payload in 
-           lemma_eq_intro bs (pad payload Handshake len);
-           Correct f
-  | 23z -> let rg:frange i = (0, j) in
-           let payload = fst (Platform.Bytes.split bs j) in
-           let d = DataStream.mk_fragment #i rg payload in
-           assert(forall (k:nat {j < k /\ k < length bs}). Seq.index bs k = 0z);
-           lemma_eq_intro bs (pad payload Application_data len);
-           Correct (CT_Data rg d)
+  match index bs j with
+  | 0z ->
+    if j > 0 then scan i bs (j-1)
+    else Error (AD_decode_error, "No ContentType byte")
+  | 21z ->
+    if j = 0 then Error (AD_decode_error, "Empty Alert fragment")
+    else
+      if j > max_TLSPlaintext_fragment_length then
+	Error (AD_record_overflow, "TLSPlaintext fragment exceeds maximum length")
+      else
+	let rg:frange i = (0, j) in
+	let payload, _ = Platform.Bytes.split bs j in
+	let f = CT_Alert rg payload in
+        lemma_eq_intro bs (pad payload Alert len);
+        Correct f
+  | 22z ->
+    if j = 0 then Error (AD_decode_error, "Empty Handshake fragment")
+    else
+      if j > max_TLSPlaintext_fragment_length then
+	Error (AD_record_overflow, "TLSPlaintext fragment exceeds maximum length")
+      else
+	let rg:frange i = (0, j) in
+	let payload, _ = Platform.Bytes.split bs j in
+	let f = CT_Handshake rg payload in
+        lemma_eq_intro bs (pad payload Handshake len);
+        Correct f
+  | 23z -> 
+    if j > max_TLSPlaintext_fragment_length then
+      Error (AD_record_overflow, "TLSPlaintext fragment exceeds maximum length")
+    else
+      let rg:frange i = (0, j) in
+      let payload, _ = Platform.Bytes.split bs j in
+      let d = DataStream.mk_fragment #i rg payload in // REMARK: No-op
+      let f = CT_Data rg d in
+      lemma_eq_intro bs (pad payload Application_data len);
+      Correct f
   | _    -> Error (AD_decode_error, "") 
 
 
@@ -107,10 +113,11 @@ let mk_plain i l pr =
   | Correct p -> Some p
   | Error _ -> None
 
-(*  OLD VERSION, breaking abstraction:
-    let len = (length pr) - 1 in
-    let (p,ctb) = Platform.Bytes.split pr len in
-    match Content.parseCT ctb with
-    | Correct ct -> Some (Content.mk_fragment i ct (0,len) p)
-    | Error z -> None
+(* OLD VERSION, breaking abstraction:
+let mk_plain i l pr =
+  let len = (length pr) - 1 in
+  let (p,ctb) = Platform.Bytes.split pr len in
+  match Content.parseCT ctb with
+  | Correct ct -> Some (Content.mk_fragment i ct (0,len) p)
+  | Error z -> None
 *)
